<?xml version="1.0"?>


<!DOCTYPE rdf:RDF [
    <!ENTITY mo "http://purl.org/ontology/mo/" >
    <!ENTITY owl "http://www.w3.org/2002/07/owl#" >
    <!ENTITY ontology "http://grasstunes.net/ontology/" >
    <!ENTITY xsd "http://www.w3.org/2001/XMLSchema#" >
    <!ENTITY owl2xml "http://www.w3.org/2006/12/owl2-xml#" >
    <!ENTITY rdfs "http://www.w3.org/2000/01/rdf-schema#" >
    <!ENTITY rdf "http://www.w3.org/1999/02/22-rdf-syntax-ns#" >
    <!ENTITY classicalmusicnav "http://purl.org/ontology/classicalmusicnav#" >
]>


<rdf:RDF xmlns="http://purl.org/ontology/classicalmusicnav#"
     xml:base="http://purl.org/ontology/classicalmusicnav"
     xmlns:classicalmusicnav="http://purl.org/ontology/classicalmusicnav#"
     xmlns:rdfs="http://www.w3.org/2000/01/rdf-schema#"
     xmlns:owl2xml="http://www.w3.org/2006/12/owl2-xml#"
     xmlns:mo="http://purl.org/ontology/mo/"
     xmlns:owl="http://www.w3.org/2002/07/owl#"
     xmlns:xsd="http://www.w3.org/2001/XMLSchema#"
     xmlns:rdf="http://www.w3.org/1999/02/22-rdf-syntax-ns#"
     xmlns:ontology="http://grasstunes.net/ontology/">
    <owl:Ontology rdf:about="">
        <rdfs:comment xml:lang="en"
            >This ontology provides a vocabulary for describing influence relationships between classical music composers.  The inspiration for this ontology was to bring the network of classical composer influence as specified by by Charles H. Smith et al. in the Classical Music Navigator -  http://www.wku.edu/~smithch/music/index2.htm</rdfs:comment>
    </owl:Ontology>
    


    <!-- 
    ///////////////////////////////////////////////////////////////////////////////////////
    //
    // Object Properties
    //
    ///////////////////////////////////////////////////////////////////////////////////////
     -->

    


    <!-- http://purl.org/ontology/classicalmusicnav#from_style_period -->

    <owl:ObjectProperty rdf:about="#from_style_period">
        <rdfs:comment xml:lang="en"
            >Style/Period: Information in this field relays primary (and sometimes secondary) stylistic and period affinities.</rdfs:comment>
        <rdfs:domain rdf:resource="#Composer"/>
        <rdfs:range rdf:resource="#StylePeriod"/>
        <rdfs:domain rdf:resource="&mo;Composer"/>
    </owl:ObjectProperty>
    


    <!-- http://purl.org/ontology/classicalmusicnav#hasInfluenced -->

    <owl:ObjectProperty rdf:about="#hasInfluenced">
        <rdfs:comment xml:lang="en"
            >The Classical Music Navigator has influenced relationship.  For example, Claude DeBussy cmn:hasInfluenced Igor Stravinsky

From the original website:
Has Influenced: Lists individuals and groups influenced BY a given composer. Names that appear IN CAPS represent major, even dominating, influences. Additional enhancement regarding time lags is again provided by plus and minus signs: &#39;-&#39; indicates that the composer influenced is older than the subject composer; no designation indicates that the subject composer is older than the composer influenced, but was alive during the latter&#39;s lifetime; &#39;+&#39; indicates that the composer influenced was born 0 to 25 years after the subject composer&#39;s death; &#39;++&#39; indicates that the composer influenced was born 25 to 100 years after the subject composer&#39;s death; &#39;+++&#39; indicates that the composer influenced was born at least 100 years after the subject composer&#39;s death.</rdfs:comment>
        <rdfs:range rdf:resource="#Composer"/>
        <rdfs:domain rdf:resource="#Composer"/>
        <rdfs:domain rdf:resource="&mo;Composer"/>
        <rdfs:range rdf:resource="&mo;Composer"/>
    </owl:ObjectProperty>
    


    <!-- http://purl.org/ontology/classicalmusicnav#influencedBy -->

    <owl:ObjectProperty rdf:about="#influencedBy">
        <rdfs:comment xml:lang="en"
            >The Classical Music Navigator influenced by relationship.  For example, Claude DeBussy cmn:influencedBy Fryderyk Chopin.

From the original website:
Musical Influences: Lists individual and group musical influences ON a given composer. Names that appear IN CAPS represent major, even dominating, influences. An additional enhancement employing plus and minus signs before the influence&#39;s name conveys information on the time lag of influence involved. Thus, a &#39;---&#39; designation indicates that that composer died (or disappeared, in the case of group influences) at least 100 years before the subject composer was born; &#39;--&#39; indicates a death 25 to 100 years before the subject composer was born; &#39;-&#39; indicates a death 0 to 25 years before the subject composer was born; no designation indicates that the influencing composer was older than the subject composer, but alive during the latter&#39;s lifetime; &#39;+&#39; indicates that the influencing composer was actually younger than the subject composer.</rdfs:comment>
        <rdfs:domain rdf:resource="#Composer"/>
        <rdfs:range rdf:resource="#Composer"/>
        <rdfs:domain rdf:resource="&mo;Composer"/>
        <rdfs:range rdf:resource="&mo;Composer"/>
    </owl:ObjectProperty>
    


    <!-- http://purl.org/ontology/classicalmusicnav#quantity_of_work_produced -->

    <owl:ObjectProperty rdf:about="#quantity_of_work_produced">
        <rdfs:comment xml:lang="en"
            >Quantity of Work Produced: This field has also been prepared for the top 222 rated composers only; it describes in general terms the absolute quantity of musical output by the composer by assigning one of five ratings in the ascending order: &#39;small,&#39; &#39;modest,&#39; &#39;considerable,&#39; &#39;extensive,&#39; and &#39;immense.&#39;</rdfs:comment>
        <rdfs:domain rdf:resource="#Composer"/>
        <rdfs:range rdf:resource="#Composer"/>
        <rdfs:range rdf:resource="#WorkQuantity"/>
        <rdfs:domain rdf:resource="&mo;Composer"/>
    </owl:ObjectProperty>
    


    <!-- 
    ///////////////////////////////////////////////////////////////////////////////////////
    //
    // Data properties
    //
    ///////////////////////////////////////////////////////////////////////////////////////
     -->

    


    <!-- http://purl.org/ontology/classicalmusicnav#genre_profile -->

    <owl:DatatypeProperty rdf:about="#genre_profile">
        <rdfs:comment xml:lang="en"
            >Genre Profile: This field attempts to provide a shorthand &#39;profile&#39; of the relative importance of the composer&#39;s output as divided up into nineteen &#39;genre categories.&#39; The profile itself appears graphically as nineteen digits, grouped into six supercategories. The nineteen genre categories so grouped are as follows:

     1a. Symphonies
     1b. Orchestral: From Stage
     1c. Orchestral: Self-Standing

     2a. Single Featured Instrument &amp; Orchestra: Keyboard Instruments
     2b. Single Featured Instrument &amp; Orchestra: Violin, Cello or Viola
     2c. Single Featured Instrument &amp; Orchestra: Other
     2d. Featured Instrument &amp; Orchestra: Multiple Instruments/Concerti Grossi

     3a. Chamber Music: Five to Nine Players
     3b. Chamber Music: Four Players
     3c. Chamber Music: Three Players
     3d. Chamber Music: Two Players

     4a. Works for Solo Piano
     4b. Works for Other Solo Keyboard Instruments
     4c. Works for Other Solo Instruments

     5a. Ballets
     5b. Operas &amp; Operettas

     6a. Sacred Vocal/Choral Music
     6b. Secular Vocal/Choral Music
     6c. Electronics-Based Music

These groupings, it should be noted, represent the same main categories into which the &quot;Basic Library&quot; file is divided. On each of these genres the output of the composer is rated on a 0-3 scale, where &#39;0&#39; means &quot;did not compose in this genre,&quot; &#39;1&#39; means &quot;produced work of only minor import,&quot; &#39;2&#39; means &quot;produced significant work,&quot; and &#39;3&#39; means &quot;produced work of major musical import.&quot; The ratings are subjectively assessed, and could be quibbled over, but in general the difference between a &#39;1&#39; and a &#39;3,&#39; at least, should be fairly obvious. Importantly, only the 222 highest-rated composers have been assessed in this fashion; further, from these 222 only composers primarily active after about 1700 have been profiled.

So, a profile that visually appears as: &#39;303-2222-1112-111-00-11x&#39; would signify a composer who produced important symphonies and orchestral pieces (but no orchestral overtures or the like from stage works), a series of moderately important works for various featured instruments and orchestra, minor chamber music works (except for some successful works for two instruments), minor works for solo instruments, no ballets or operas or operettas, minor works for voice, and some electronic music (the last being unscaled here and, when present, indicated with an &#39;x&#39;).</rdfs:comment>
        <rdfs:domain rdf:resource="#Composer"/>
        <rdfs:domain rdf:resource="&mo;Composer"/>
        <rdfs:range rdf:resource="&xsd;string"/>
    </owl:DatatypeProperty>
    


    <!-- http://purl.org/ontology/classicalmusicnav#geographical_affinities -->

    <owl:DatatypeProperty rdf:about="#geographical_affinities">
        <rdfs:comment xml:lang="en"
            >Geographical Affinities: The first line of each record gives the composer&#39;s name (including less frequently used middle names given in parentheses, and alternate language names given in brackets), his or her year of birth (and year of death, if deceased), and applicable geographical affinities.</rdfs:comment>
        <rdfs:domain rdf:resource="#Composer"/>
        <rdfs:domain rdf:resource="&mo;Composer"/>
        <rdfs:range rdf:resource="&xsd;string"/>
    </owl:DatatypeProperty>
    


    <!-- http://purl.org/ontology/classicalmusicnav#notable_works -->

    <owl:DatatypeProperty rdf:about="#notable_works">
        <rdfs:comment
            >Notable Works:  This field lists in chronological order (as much as is possible) compositions by the composer that are outstanding. Here, &quot;outstanding&quot; is defined in terms of music in general, and not the output of any one composer. The result is that quite a few composers on the list are not distinguished in this fashion; these are individuals who may have created a solid body of work from which no individual piece stands out. It should be noted the &#39;Best Known For&#39; and &#39;Notable Works&#39; fields are combined for some composers into a single &#39;Best Known Work&#39; field, as convenient.</rdfs:comment>
        <rdfs:domain rdf:resource="#Composer"/>
        <rdfs:domain rdf:resource="&mo;Composer"/>
        <rdfs:range rdf:resource="&xsd;string"/>
    </owl:DatatypeProperty>
    


    <!-- 
    ///////////////////////////////////////////////////////////////////////////////////////
    //
    // Classes
    //
    ///////////////////////////////////////////////////////////////////////////////////////
     -->

    


    <!-- http://purl.org/ontology/classicalmusicnav#Composer -->

    <owl:Class rdf:about="#Composer">
        <owl:equivalentClass rdf:resource="&mo;Composer"/>
        <rdfs:subClassOf rdf:resource="&mo;Composer"/>
        <rdfs:comment xml:lang="en"
            >A composer of music</rdfs:comment>
    </owl:Class>
    


    <!-- http://purl.org/ontology/classicalmusicnav#StylePeriod -->

    <owl:Class rdf:about="#StylePeriod">
        <rdfs:subClassOf rdf:resource="&owl;Thing"/>
        <rdfs:comment xml:lang="en"
            >Style/Period: Information in this field relays primary (and sometimes secondary) stylistic and period affinities.</rdfs:comment>
    </owl:Class>
    


    <!-- http://purl.org/ontology/classicalmusicnav#WorkQuantity -->

    <owl:Class rdf:about="#WorkQuantity">
        <rdfs:subClassOf rdf:resource="&owl;Thing"/>
        <rdfs:comment xml:lang="en"
            >Quantity of Work Produced: This field has also been prepared for the top 222 rated composers only; it describes in general terms the absolute quantity of musical output by the composer by assigning one of five ratings in the ascending order: &#39;small,&#39; &#39;modest,&#39; &#39;considerable,&#39; &#39;extensive,&#39; and &#39;immense.&#39;</rdfs:comment>
    </owl:Class>
    


    <!-- http://purl.org/ontology/classicalmusicnavWorkQuantity -->

    <owl:Class rdf:about="WorkQuantity"/>
    


    <!-- http://purl.org/ontology/mo/Composer -->

    <owl:Class rdf:about="&mo;Composer">
        <rdfs:comment xml:lang="en"
            >A Composer of music</rdfs:comment>
    </owl:Class>
    


    <!-- http://www.w3.org/2002/07/owl#Thing -->

    <owl:Class rdf:about="&owl;Thing"/>
    


    <!-- 
    ///////////////////////////////////////////////////////////////////////////////////////
    //
    // Individuals
    //
    ///////////////////////////////////////////////////////////////////////////////////////
     -->

    


    <!-- http://purl.org/ontology/classicalmusicnav#considerable -->

    <ontology:classicalmusicnav.owlWorkQuantity rdf:about="#considerable">
        <rdfs:comment
            >Quantity of Work Produced: This field has also been prepared for the top 222 rated composers only; it describes in general terms the absolute quantity of musical output by the composer by assigning one of five ratings in the ascending order: &#39;small,&#39; &#39;modest,&#39; &#39;considerable,&#39; &#39;extensive,&#39; and &#39;immense.&#39;</rdfs:comment>
    </ontology:classicalmusicnav.owlWorkQuantity>
    


    <!-- http://purl.org/ontology/classicalmusicnav#extensive -->

    <ontology:classicalmusicnav.owlWorkQuantity rdf:about="#extensive">
        <rdfs:comment
            >Quantity of Work Produced: This field has also been prepared for the top 222 rated composers only; it describes in general terms the absolute quantity of musical output by the composer by assigning one of five ratings in the ascending order: &#39;small,&#39; &#39;modest,&#39; &#39;considerable,&#39; &#39;extensive,&#39; and &#39;immense.&#39;</rdfs:comment>
    </ontology:classicalmusicnav.owlWorkQuantity>
    


    <!-- http://purl.org/ontology/classicalmusicnav#immense -->

    <ontology:classicalmusicnav.owlWorkQuantity rdf:about="#immense">
        <rdfs:comment
            >Quantity of Work Produced: This field has also been prepared for the top 222 rated composers only; it describes in general terms the absolute quantity of musical output by the composer by assigning one of five ratings in the ascending order: &#39;small,&#39; &#39;modest,&#39; &#39;considerable,&#39; &#39;extensive,&#39; and &#39;immense.&#39;</rdfs:comment>
    </ontology:classicalmusicnav.owlWorkQuantity>
    


    <!-- http://purl.org/ontology/classicalmusicnav#modest -->

    <ontology:classicalmusicnav.owlWorkQuantity rdf:about="#modest">
        <rdfs:comment
            >Quantity of Work Produced: This field has also been prepared for the top 222 rated composers only; it describes in general terms the absolute quantity of musical output by the composer by assigning one of five ratings in the ascending order: &#39;small,&#39; &#39;modest,&#39; &#39;considerable,&#39; &#39;extensive,&#39; and &#39;immense.&#39;</rdfs:comment>
    </ontology:classicalmusicnav.owlWorkQuantity>
    


    <!-- http://purl.org/ontology/classicalmusicnav#small -->

    <ontology:classicalmusicnav.owlWorkQuantity rdf:about="#small">
        <rdfs:comment
            >Quantity of Work Produced: This field has also been prepared for the top 222 rated composers only; it describes in general terms the absolute quantity of musical output by the composer by assigning one of five ratings in the ascending order: &#39;small,&#39; &#39;modest,&#39; &#39;considerable,&#39; &#39;extensive,&#39; and &#39;immense.&#39;</rdfs:comment>
    </ontology:classicalmusicnav.owlWorkQuantity>
</rdf:RDF>



<!-- Generated by the OWL API (version 2.2.1.962) http://owlapi.sourceforge.net -->

